Added 2 more VCs to json

compositionality/Json/Json.fst
@@ -88,36 +88,8 @@ let merge_idem_b s = ()
 
 ////////////////////////////////////////////////////////////////////////////
 
-let base_2op_a o1 o2 = ()
-let base_2op_b o1 o2 = ()
-let base_2op' o1 o2 t = ()
-
-#set-options "--z3rlimit 200 --ifuel 3"
-let ind_lca_2op_a l o1 o2 ol = ()
-let ind_lca_2op_b l o1 o2 ol = ()
-let ind_lca_2op' l o1 o2 ol = ()
-
-let inter_right_base_2op_a l a b o1 o2 ob ol = ()
-let inter_right_base_2op_b l a b o1 o2 ob ol = ()
-let inter_right_base_2op' l a b o1 o2 ob ol = ()
-
-let inter_left_base_2op_a l a b o1 o2 ob ol = ()
-let inter_left_base_2op_b l a b o1 o2 ob ol = ()
-let inter_left_base_2op' l a b o1 o2 ob ol = ()
-
-let inter_right_2op_a l a b o1 o2 ob ol o = ()
-let inter_right_2op_b l a b o1 o2 ob ol o = ()
-let inter_right_2op' l a b o1 o2 ob ol o = ()
-
-let inter_left_2op_a l a b o1 o2 ob ol o = ()
-let inter_left_2op_b l a b o1 o2 ob ol o = ()
-let inter_left_2op' l a b o1 o2 ob ol o = ()
-
-let ind_right_2op_a l a b o1 o2 o2' = ()
-let ind_right_2op_b l a b o1 o2 o2' = ()
-
-let ind_left_2op_a l a b o1 o2 o1' = ()
-let ind_left_2op_b l a b o1 o2 o1' = ()
+let lem_0op_a l a b ol = ()
+let lem_0op_b l a b ol = ()
 
 let base_1op_a o1 = ()
 let base_1op_b o1 = ()
@@ -137,6 +109,9 @@ let inter_right_1op_b l a b o1 ob ol o = ()
 let inter_left_1op_a l a b o1 ob ol o = ()
 let inter_left_1op_b l a b o1 ob ol o = ()
 
+let inter_lca_1op_a l a b o1 ol oi o = ()
+let inter_lca_1op_b l a b o1 ol oi o = ()
+
 let ind_right_1op_a l a b o1 o1' ol = ()
 let ind_right_1op_b l a b o1 o1' ol = ()
 let ind_right_1op' l a b o1 o1' ol = ()
@@ -145,5 +120,32 @@ let ind_left_1op_a l a b o1 o1' ol = ()
 let ind_left_1op_b l a b o1 o1' ol = ()
 let ind_left_1op' l a b o1 o1' ol = ()
 
-let lem_0op_a l a b ol = ()
-let lem_0op_b l a b ol = ()
+let base_2op_a o1 o2 = ()
+let base_2op_b o1 o2 = ()
+
+let ind_lca_2op_a l o1 o2 ol = ()
+let ind_lca_2op_b l o1 o2 ol = ()
+
+let inter_right_base_2op_a l a b o1 o2 ob ol = ()
+let inter_right_base_2op_b l a b o1 o2 ob ol = ()
+
+let inter_left_base_2op_a l a b o1 o2 ob ol = ()
+let inter_left_base_2op_b l a b o1 o2 ob ol = ()
+
+let inter_right_2op_a l a b o1 o2 ob ol o = ()
+let inter_right_2op_b l a b o1 o2 ob ol o = ()
+
+let inter_left_2op_a l a b o1 o2 ob ol o = ()
+let inter_left_2op_b l a b o1 o2 ob ol o = ()
+
+let inter_lca_2op_a l a b o1 o2 ol o = ()
+let inter_lca_2op_b l a b o1 o2 ol o = ()
+let inter_lca_2op' l a b o1 o2 ol o = ()
+
+let ind_right_2op_a l a b o1 o2 o2' = ()
+let ind_right_2op_b l a b o1 o2 o2' = ()
+
+let ind_left_2op_a l a b o1 o2 o1' = ()
+let ind_left_2op_b l a b o1 o2 o1' = ()
+let ind_left_2op' l a b o1 o2 o1' = ()
+
